theories/L/AbstractMachines/Computable/UnivDecTime.v
@@ -1,5 +1,5 @@
 From Undecidability.L.Datatypes Require Import LNat LBool.
-From Undecidability.L Require Import Tactics.LTactics  Prelim.LoopSum Functions.UnboundIteration AbstractMachines.LargestVar.
+From Undecidability.L Require Import Util.Subterm Tactics.LTactics  Prelim.LoopSum Functions.UnboundIteration AbstractMachines.LargestVar.
 From Complexity.L Require Import AbstractMachines.Computable.Unfolding.
 From Complexity.L.AbstractMachines Require Import AbstractHeapMachine FunctionalDefinitions UnfoldHeap UnfoldTailRec. 
 From Complexity.L.AbstractMachines.Computable Require Import Shared HeapMachine Unfolding.
