theories/L/AbstractMachines/FlatPro/SubtermProperty.v
@@ -1,0 +1,155 @@
+From Undecidability Require Import TM.Util.TM_facts TM.Util.Relations.
+From Undecidability.L Require Import Util.Subterm Util.L_facts.
+From Undecidability.L Require Import LM_heap_def.
+From Complexity Require Import FlatPro.SizeAnalysisStep.
+
+Set Default Proof Using "Type".
+Require Import FunInd.
+
+Import L_Notations.
+
+
+Inductive taskOf : L.term -> Pro -> Prop :=
+| taskVar x: taskOf (L.var x) (compile (L.var x))
+| taskLam s: taskOf (L.lam s) (compile (L.lam s))
+| taskL (s t:L.term) P : taskOf s P -> taskOf (s t) (P++compile t++[appT])
+| taskR (s t:term) P: taskOf t P -> taskOf (s t) (P++[appT])
+| taskAppT (s t:term): taskOf (s t) ([appT]).
+
+Lemma taskOf_refl s : taskOf s (compile s).
+Proof. induction s;cbn. 1,3:constructor. now apply taskL. Qed.   
+
+Lemma taskOf_notNil s: ~ taskOf s [].
+Proof. intros H. remember [] as P eqn:HP. induction H in H,HP|-*;cbn in *. 1,2,5:easy. 1,2:now destruct P. Qed.  
+
+
+Lemma taskOf_jumpTarget s P :
+  taskOf s (lamT::P) ->
+  exists s' P', (P =compile s' ++ retT ::P') /\ subterm (lam s') s /\ (P'=[] \/ taskOf s P').
+Proof.
+  intros H. remember (lamT::P) as P0 eqn:HP0. revert P HP0. induction H.
+  - easy.
+  - cbn. intros ? [= <-]. do 2 eexists. split. reflexivity. split. easy. easy.
+  - intros P0 HP. destruct P. now edestruct taskOf_notNil. inv HP.
+    edestruct IHtaskOf as (s'&P'&HP&Hs'&H''). reflexivity. subst P.
+    do 2 eexists. split. rewrite <- app_assoc;cbn. reflexivity.
+    split. now eauto using subterm.
+    all:right. destruct H'' as [->|?];cbn. 2:now eauto using taskOf.
+    econstructor. apply taskOf_refl.
+  - intros P0 HP. destruct P. easy. inv HP.
+    edestruct IHtaskOf as (s'&P'&HP&Hs'&H''). reflexivity. subst P.
+    do 2 eexists. split. now (rewrite <- app_assoc;cbn).
+    split. now eauto using subterm.
+    all:right. destruct H'' as [->|?];cbn. 2:now eauto using taskOf. now econstructor.
+  - easy. 
+Qed. 
+
+
+Lemma taskOf_appT s P :
+  taskOf s (appT::P) ->
+  P = [] \/ taskOf s P.
+Proof.
+  intros H. remember (appT::P) as P0 eqn:HP0. revert P HP0. induction H.
+  - easy.
+  - easy.
+  - intros P0 HP. destruct P. now edestruct taskOf_notNil. inv HP.
+    specialize IHtaskOf with (1:=eq_refl) as [->|];cbn. all:right;eauto using taskOf,taskOf_refl. 
+  - intros P0 HP. destruct P. inv HP.  easy. inv HP.
+    edestruct IHtaskOf as [IH|IH]. reflexivity. subst P.  all:right;eauto using taskOf,taskOf_refl.
+  - now left. 
+Qed. 
+
+
+Lemma taskOf_varT s P n :
+  taskOf s (varT n::P) ->
+  P = [] \/ taskOf s P.
+Proof.
+  intros H. remember (varT n::P) as P0 eqn:HP0. revert P HP0. induction H.
+  - cbv. intros ? [= ->]. easy.
+  - easy.
+  - intros P0 HP. destruct P. now edestruct taskOf_notNil. inv HP.
+    specialize IHtaskOf with (1:=eq_refl) as [->|];cbn. all:right;eauto using taskOf,taskOf_refl. 
+  - intros P0 HP. destruct P. inv HP. inv HP.
+    edestruct IHtaskOf as [IH|IH]. reflexivity. subst P.  all:right;eauto using taskOf,taskOf_refl.
+  - now left. 
+Qed. 
+
+Section Analysis.
+
+  Variable T V : list HClos.
+  Variable H: list HEntr.
+
+  
+  Variable i : nat.
+
+  Variable s : L.term.
+  Hypothesis R: pow step i (init s) (T,V,H).
+
+  Import Lia.
+  
+  Lemma subterm_property :
+  (forall g, g el T -> exists s', subterm s' s /\ taskOf s' (snd g))
+   /\ (forall g, g el V -> exists s', subterm (lam s') s /\ snd g = compile s')
+   /\ (forall g beta, Some (g,beta) el H -> exists s', subterm (lam s') s /\ snd g = compile s').
+  Proof using R.
+    induction i in T,V,H,R|-*.
+    {
+      inv R. split. 2:easy. 
+      intros ? [[= <-]|[]];cbn. 
+      eauto 10 using Nat.le_0_l, taskOf_refl, (@reflexivity _ subterm _ s).
+    }
+    - replace (S n) with (n + 1) in R by lia. apply pow_add in R. destruct R as [[[T' V'] H'] [R1 R2]].
+      specialize (IHn _ _ _ R1).
+      eapply rcomp_1 in R2.
+      destruct IHn as (IHT&IHV&IHH).
+      inv R2.
+      + destruct (IHT (a,lamT::P)) as (s'&Hs'&HP). easy. cbn [fst snd] in *.
+        eapply taskOf_jumpTarget in HP as (s''&tmp&->&Hsubterm&HP').
+        rewrite jumpTarget_correct in H2. injection H2 as [= <- ->].
+
+        destruct P',HP'. 3:easy. 2:now edestruct taskOf_notNil.
+        all:split;[intros g|split;[intros g|intros g beta]].
+        all:intros Hg;cbn in Hg;try decompose [or] Hg.
+        all:eauto. all:subst;cbn [fst snd] in *.
+        2:easy.
+        all:eexists. all:split;[|reflexivity]. 
+        { etransitivity. 2:eassumption. eauto using subterm, (@reflexivity _ subterm _ s). } 
+        { etransitivity. 2:eassumption. eauto using subterm, (@reflexivity _ subterm _ s). }
+      + destruct (IHT (a,appT::P)) as (s'&Hsubterm&HP). easy. cbn [fst snd] in *.
+        eapply taskOf_appT in HP as HP'.
+        injection H2 as [= <- <-]. 
+
+        all:split;[intros g'|split;[intros g'|intros g' beta]].
+        1:destruct P,HP'. 3:easy. 2:now edestruct taskOf_notNil.
+        all:intros Hg;cbn in Hg;try decompose [or] Hg.  
+        { 
+          edestruct IHV as (?&IHV'). now right;left. destruct IHV' as (?&[= ->]). subst g'.
+          do 2 eexists. 2:apply taskOf_refl. 
+          etransitivity. 2:eassumption. eauto using subterm, (@reflexivity _ subterm _ s).
+        }
+        all:eauto.
+        { subst g'.
+          edestruct IHV as (?&IHV'). now right;left. destruct IHV' as (?&[= ->]).
+          do 2 eexists. 2:apply taskOf_refl. 
+          etransitivity. 2:eassumption. eauto using subterm, (@reflexivity _ subterm _ s).
+        }
+        {subst g'. eauto. }
+        eapply in_app_or in Hg as []. eauto. cbn in H.
+        destruct H as [[= <- <-]|[]].
+        edestruct (IHV g) as (?&?&?). easy.
+        edestruct (IHV (b,Q)) as (?&?&?). easy.
+        eauto.
+      + eapply lookup_el in H2 as (?&Hg).
+        destruct (IHH _ _ Hg) as (?&?&?).
+        destruct (IHT (a,varT n0::P)) as (s'&Hsubterm&HP). easy. cbn [fst snd] in *.
+        eapply taskOf_varT in HP.
+
+        all:split;[intros g'|split;[intros g'|intros g' beta]].
+        1:destruct P,HP. 3:easy. 2:now edestruct taskOf_notNil.
+        all:intros Hg';cbn in Hg';try decompose [or] Hg'.
+        all:eauto.  
+        { subst g';cbn. easy. }
+        { subst g'. easy. }
+  Qed.
+
+End Analysis.
